Dpss.lean
@@ -35,6 +35,7 @@ import Dpss.IntModel
 import Dpss.Fence
 import Dpss.FenceInt
 import Dpss.FenceTrace
+import Dpss.SeparationInt
 import Dpss.Standoff
 import Dpss.Separation
 import Dpss.Kinematics
